PQueueA : atomic specification Incr : merge incr_cas and incr_faa into a single example

incr/ClientI.v
@@ -1,15 +1,16 @@
 Require Import CRIS.
 Require Import ImpPrelude MemHeader SchHeader.
-Require Import FaaHeader.
+Require Import IncrHeader.
 
 Module ClientI. Section ClientI.
   Context `{!crisG Γ Σ α β τ _S _I}.
 
   Definition scopes : list string := [].
 
-  Definition incr : list val → itree crisE unit :=
+  Definition thread : list val → itree crisE unit :=
     λ arg,
-      𝒴;;; '_ : unit <- ccallU FaaHdr.faa2 arg;;
+      𝒴;;; '_ : val <- ccallU IncrHdr.incr arg;;
+      𝒴;;; '_ : val <- ccallU IncrHdr.incr arg;;
       𝒴;;; Ret tt.
 
   Definition main : Any.t → itree crisE Any.t :=
@@ -17,17 +18,17 @@ Module ClientI. Section ClientI.
       𝒴;;; 'ptr_raw : val <- ccallU MemHdr.alloc [Vint 1%Z];;
       𝒴;;; bofs <- (pargs [Tptr] [ptr_raw])?;;
       𝒴;;; '_ : val <- ccallU MemHdr.store [Vptr bofs; Vint 0%Z];;
-      𝒴;;; tid1 <- Sch.spawn (IncrHdr.incr, [Vptr bofs]↑↑);;
-      𝒴;;; tid2 <- Sch.spawn (IncrHdr.incr, [Vptr bofs]↑↑);;
+      𝒴;;; tid1 <- Sch.spawn (ClientHdr.thread, [Vptr bofs]↑↑);;
+      𝒴;;; tid2 <- Sch.spawn (ClientHdr.thread, [Vptr bofs]↑↑);;
       𝒴;;; Sch.join tid1;;;
       𝒴;;; Sch.join tid2;;;
       𝒴;;; 'v_raw : val <- ccallU MemHdr.load [Vptr bofs];;
       𝒴;;; 'v : Z <- (pargs [Tint] [v_raw])?;;
-      𝒴;;; '_ : unit <- trigger (IO "OUT" v);;
+      𝒴;;; '_ : val <- trigger (IO "OUT" v);;
       𝒴;;; Ret (tt↑).
 
   Definition fnsems : fnsemmap :=
-    {[fid IncrHdr.incr # (msk_real (msk_scp scopes msk_true), (None, cfunU (sfunU incr)));
+    {[fid ClientHdr.thread # (msk_real (msk_scp scopes msk_true), (None, cfunU (sfunU thread)));
       entry # (msk_real (msk_scp scopes msk_true), (None, main))]}.
 
   Program Definition smod : SMod.t := {|
