incr/IncrA.v
@@ -1,0 +1,34 @@
+Require Import CRIS Atomic.
+Require Import ImpPrelude.
+Require Import SchHeader SchA.
+Require Import MemHeader MemA.
+Require Import IncrHeader.
+
+Module IncrA. Section IncrA.
+  Context `{!crisG Γ Σ α β τ _S _I, !memGS, !concGS}.
+
+  Definition scopes : list string := [].
+
+  Definition incr_spec : fspec_atomic := {|
+    meta_priv := mblock * ptrofs;
+    meta_pub := Z;
+    pre_priv := λ bofs arg, ⌜arg = [Vptr bofs]↑⌝;
+    pre_pub := λ bofs v _, bofs ↦ Vint v;
+    post_pub := λ bofs v ret, bofs ↦ Vint (v + 1);
+    post_priv := λ bofs v ret, ⌜ret = (Vint v)↑⌝;
+  |}%I.
+
+  Definition fnsems : fnsemmap :=
+    {[fid IncrHdr.incr #
+        (msk_scp scopes msk_true,
+          (None, atomic_fun incr_spec (atomic_update incr_spec)))]}.
+
+  Program Definition smod : SMod.t := {|
+    SMod.scopes := scopes;
+    SMod.fnsems := fnsems;
+    SMod.initial_st := ∅;
+  |}.
+  Solve All Obligations with mod_tac.
+
+  Definition t : Mod.t := SMod.to_mod ∅ smod.
+End IncrA. End IncrA.
