incr/IncrHeader.v
@@ -1,0 +1,9 @@
+Require Import Common.
+
+Module IncrHdr.
+  Definition incr := "incr".
+End IncrHdr.
+
+Module ClientHdr.
+  Definition thread := "thread".
+End ClientHdr.
