incr/IncrIAproof.v
@@ -1,0 +1,46 @@
+Require Import CRIS Atomic.
+Require Import SchHeader SchA SchTactics.
+Require Import ImpPrelude MemHeader MemA MemTactics.
+Require Import IncrHeader IncrI IncrA.
+
+Module IncrIA. Section IncrIA.
+  Context `{!crisG Γ Σ α β τ _S _I, !memGS, !concGS, !schGS}.
+  Context (sp : specmap).
+
+  Local Definition IstFull := (IstProd (IstSB (Mod.scopes (IncrA.t)) IstTrue) IstEq).
+  Local Notation MA := (IncrA.t ★ (MemA.t sp)).
+  Local Notation MI := (IncrI.t ★ (MemA.t sp)).
+
+  Lemma incr_simF : ISim.sim_fun open MA MI IstFull (fid IncrHdr.incr).
+  Proof.
+    cStartFunSim. cStepsS. cStepsT. iApply atomic_fun_src.
+    iIntros ([blk ofs]) "->". rewrite /IncrI.incr unfold_atomic_update. cStepsT. cStepsS.
+
+    sYieldRR "IST". sYieldRR "IST".
+
+    iApply wsim_reset.
+    cCoind CIH g __ with st_src st_tgt.
+    iIntros "IST /=".
+
+    unfoldIterCT. cStepsT. sYieldRR "IST". sYieldS. cStepsS.
+    rename _q into v; iRename "ASM" into "↦".
+    mLoadT "↦". cForceS (inl tt); cForcesS; iFrame "↦". cStepsS.
+    rewrite unfold_atomic_update; cStepsS. sYieldRR "IST". sYieldRR "IST". sYieldS; cStepsS.
+    rename _q into v2; iRename "ASM" into "↦".
+
+    iApply (wsim_mem_cas with "↦"); [prove_inline_cond|ss|eauto| | | ].
+    { rewrite /MemA.compare_val; des_ifs. }
+    { instantiate (1:=emp%I); done. }
+    { iIntros "_"; iExists 1%Qp, 1%Qp, Vundef, Vundef; ss. }
+    iIntros "↦ _". cStepsT. case_bool_decide.
+    { case_bool_decide; subst; ss. cForceS (inr _); cForcesS; iFrame "↦".
+      cStepsS. sYieldRR "IST". sYieldRR "IST".
+      rewrite decide_True //. cStepsT. sYieldS. cStep; iFrame; iSplit; first ss.
+      cStep. iFrame. done.
+    }
+    case_bool_decide; ss. cForceS (inl tt). cForcesS; iFrame. cStepsS.
+    rewrite unfold_atomic_update; cStepsS.
+    sYieldRR "IST". sYieldRR "IST". case_decide; ss. cStepsT.
+    cByCoind CIH. iFrame.
+  (*SLOW*)Qed.
+End IncrIA. End IncrIA.
