incr_cas/IncrementHeader.v
@@ -1,5 +1,0 @@
-Require Import Common.
-
-Module IncrementHdr.
-  Definition increment := "increment".
-End IncrementHdr.
